# [780.Reaching Points](https://leetcode.com/problems/reaching-points/description/)

## Description

**Tags**: array

**Companies**: Unknown

|  Category  |  Difficulty   | Likes | Dislikes |
| :--------: | :-----------: | :---: | :------: |
| algorithms | Hard (32.87%) | 1423  |   221    |

<p>Given four integers <code>sx</code>, <code>sy</code>, <code>tx</code>, and <code>ty</code>, return <code>true</code><em> if it is possible to convert the point </em><code>(sx, sy)</code><em> to the point </em><code>(tx, ty)</code> <em>through some operations</em><em>, or </em><code>false</code><em> otherwise</em>.</p>
<p>The allowed operation on some point <code>(x, y)</code> is to convert it to either <code>(x, x + y)</code> or <code>(x + y, y)</code>.</p>
<p>&nbsp;</p>
<p><strong class="example">Example 1:</strong></p>
<pre><code><strong>Input:</strong> sx = 1, sy = 1, tx = 3, ty = 5
<strong>Output:</strong> true
<strong>Explanation:</strong>
One series of moves that transforms the starting point to the target is:
(1, 1) -&gt; (1, 2)
(1, 2) -&gt; (3, 2)
(3, 2) -&gt; (3, 5)</code></pre>
<p><strong class="example">Example 2:</strong></p>
<pre><code><strong>Input:</strong> sx = 1, sy = 1, tx = 2, ty = 2
<strong>Output:</strong> false</code></pre>
<p><strong class="example">Example 3:</strong></p>
<pre><code><strong>Input:</strong> sx = 1, sy = 1, tx = 1, ty = 1
<strong>Output:</strong> true</code></pre>
<p>&nbsp;</p>
<p><strong>Constraints:</strong></p>
<ul>
  <li><code>1 &lt;= sx, sy, tx, ty &lt;= 10<sup>9</sup></code></li>
</ul>

## Solution

**题目描述**

给定四个整数 `sx`，`sy`，`tx`，`ty`，如果通过一系列的操作可以将点 `(sx, sy)` 转变成 `(tx, ty)`，则返回 `true` 。否则，返回 `false` 。

从点 `(x, y)` 可以转变成 `(x, x+y)`  或者 `(x+y, y)`。

**解题思路**

1. 逆向转换
   - 从 `(tx, ty)` 开始逆向转换，判断是否能够转换到 `(sx, sy)`。
   - 从 `(x, y)` 可以逆向转换到 `(x-y, y)` 或者 `(x, y-x)`，所以当 `tx > ty` 时，可以转换到 `(tx-ty, ty)`，否则可以转换到 `(tx, ty-tx)`。

```cpp
class Solution {
public:
    bool reachingPoints(int sx, int sy, int tx, int ty) {
        while (tx >= sx && ty >= sy) {
            if (tx == ty) break;
            if (tx > ty) {
                if (ty > sy) tx %= ty;
                else return (tx - sx) % ty == 0;
            } else {
                if (tx > sx) ty %= tx;
                else return (ty - sy) % tx == 0;
            }
        }
        return (tx == sx && ty == sy);
    }
};
```
```
